refactor: Rename `HRel` to `Rel` (#672)

Foundation/Vorspiel/Rel/Connected.lean
@@ -1,14 +1,14 @@
-import Foundation.Vorspiel.HRel.Euclidean
-import Foundation.Vorspiel.HRel.Convergent
+import Foundation.Vorspiel.Rel.Euclidean
+import Foundation.Vorspiel.Rel.Convergent
 
-variable {α} {R : HRel α}
+variable {α} {R : Rel α α}
 
-def PiecewiseConnected (R : HRel α) := ∀ ⦃x y z⦄, R x y → R x z → (R y z ∨ y = z ∨ R z y)
+def PiecewiseConnected (R : Rel α α) := ∀ ⦃x y z⦄, R x y → R x z → (R y z ∨ y = z ∨ R z y)
 
-class IsPiecewiseConnected (R : HRel α) where
+class IsPiecewiseConnected (R : Rel α α) where
   p_connected : PiecewiseConnected R
 
-lemma IsPiecewiseConnected.p_connected' {R : HRel α} [IsPiecewiseConnected R] {x y z : α} (Rxy : R x y) (Rxz : R x z) (hyz : y ≠ z) : R y z ∨ R z y := by
+lemma IsPiecewiseConnected.p_connected' {R : Rel α α} [IsPiecewiseConnected R] {x y z : α} (Rxy : R x y) (Rxz : R x z) (hyz : y ≠ z) : R y z ∨ R z y := by
   rcases IsPiecewiseConnected.p_connected Rxy Rxz with (Ryz | rfl | Rzy) <;> tauto;
 
 instance [IsTrichotomous _ R] : IsPiecewiseConnected R :=
@@ -20,9 +20,9 @@ instance [IsRightEuclidean R] : IsPiecewiseConnected R := ⟨by
   tauto;
 ⟩
 
-def PiecewiseStronglyConnected (R : HRel α) := ∀ ⦃x y z⦄, R x y → R x z → (R y z ∨ R z y)
+def PiecewiseStronglyConnected (R : Rel α α) := ∀ ⦃x y z⦄, R x y → R x z → (R y z ∨ R z y)
 
-class IsPiecewiseStronglyConnected (R : HRel α) where
+class IsPiecewiseStronglyConnected (R : Rel α α) where
   ps_connected : PiecewiseStronglyConnected R
 
 instance [IsTotal _ R] : IsPiecewiseStronglyConnected R := ⟨fun ⦃_ y z⦄ _ _ ↦ IsTotal.total y z⟩
