Foundation/Vorspiel/Rel/Isolated.lean
@@ -1,11 +1,11 @@
-import Foundation.Vorspiel.HRel.Coreflexive
+import Foundation.Vorspiel.Rel.Coreflexive
 
-variable {α} {R : HRel α}
+variable {α} {R : Rel α α}
 
 /-- Nothing is related on `R` -/
-def Isolated (R : HRel α) := ∀ ⦃x y⦄, ¬R x y
+def Isolated (R : Rel α α) := ∀ ⦃x y⦄, ¬R x y
 
-class IsIsolated (R : HRel α) where
+class IsIsolated (R : Rel α α) where
   isolated : Isolated R
 
 @[simp] lemma isolated [IsIsolated R] {x y : α} : ¬R x y := by apply IsIsolated.isolated
